\batchmode
\documentclass{article}
\usepackage{epsfig}
\pagestyle{empty}
\begin{document}
\[ out_i = \sum_j kernel_j in_{i-j} \]
\pagebreak

$ out_i = in_{i-1}$
\pagebreak

\[ out_i = \sum_j kernel_j in_{i+j} \]
\pagebreak

\[ C_k = \sum_{i} i A_{i} \]
\pagebreak

\[ C_k = \sum_{i_1...i_n} i_k A_{i_1...i_n} \]
\pagebreak

$ {a, b, a\times b}$
\pagebreak

$ R_{ij}= \tau S_i S_j $
\pagebreak

$\tau$
\pagebreak

$\lambda$
\pagebreak

$i,j$
\pagebreak

\[ R_{ij}(t) = \tau * S_i(0) S_j(0) exp (-2 \lambda t) \]
\pagebreak

\[ r_{ij} = \tau S_i(0) S_j(0) \int_{t_1}^{t_2} dt\,exp (-2 \lambda t) \]
\pagebreak

\[ r_{ij} = \tau s_i s_j \frac{ \int_{t_1}^{t_2} dt\,exp (-2 \lambda t)}{\left(\int_{t1}^{t2} dt\,exp (-\lambda t)\right)^2} \]
\pagebreak

\[ \frac{(t_2-t_1)}{ \int_{t_1}^{t_2} \! 2^{-t/\mathrm{halflife}} \, dt} \]
\pagebreak

\[ 2^{(\mathrm{rel\_time} / \mathrm{halflife})} \]
\pagebreak

$\lambda_{ijk}$
\pagebreak

\[ \sum_{ijk} \lambda_{ijk} b_{ijk}({\bar x}) \]
\pagebreak

\[ \mu = a + b * \mathrm{HU} \]
\pagebreak

$a=a1, b=b1$
\pagebreak

$\mathrm{HI} < \mathrm{break}$
\pagebreak

$ \boldsymbol{\lambda}$
\pagebreak

$ j $
\pagebreak

$ \boldsymbol{v}_j $
\pagebreak

$\lambda_j$
\pagebreak

\[ \lambda_j= \sum_{l=1}^L \alpha_l k_{jl} \]
\pagebreak

$k_{jl}$
\pagebreak

$jl^{th}$
\pagebreak

$\boldsymbol{K}$
\pagebreak

\[ \alpha^{(n+1)}_j = \frac{ \alpha^{(n)}_j }{\sum_{m} k^{(n)}_{jm} \sum_i p_{mi}} \sum_{m}k^{(n)}_{jm}\sum_i p_{mi}\frac{ y_i }{\sum_{q} p_{iq} \sum_l k^{(n)}_{ql}\alpha^{(n)}_l + s_i} \]
\pagebreak

$ jl $
\pagebreak

\[ k^{(n)}_{jl} = k_m(\boldsymbol{v}_j,\boldsymbol{v}_l) \cdot k_p(\boldsymbol{z}^{(n)}_j,\boldsymbol{z}^{(n)}_l); \]
\pagebreak

\[ k_m(\boldsymbol{v}_j,\boldsymbol{v}_l) = \exp \left(\tiny - \frac{\| \boldsymbol{v}_j-\boldsymbol{v}_l \|^2}{2 \sigma_m^2} \right) \exp \left(- \frac{\tiny \| \boldsymbol{x}_j-\boldsymbol{x}_l \|^2}{ \tiny 2 \sigma_{dm}^2} \right) \]
\pagebreak

\[ k_p(\boldsymbol{z}^{(n)}_j,\boldsymbol{z}^{(n)}_l) = \exp \left(\tiny - \frac{\| \boldsymbol{z}^{(n)}_j-\boldsymbol{z}^{(n)}_l \|^2}{2 \sigma_p^2} \right) \exp \left(\tiny - \frac{\| \boldsymbol{x}_j-\boldsymbol{x}_l \|^2}{ \tiny{2 \sigma_{dp}^2}} \right) \]
\pagebreak

$ \| \boldsymbol{z}^{(n)}_j-\boldsymbol{z}^{(n)}_l \| $
\pagebreak

$[0,2\pi)$
\pagebreak

\[ r_s = \sum_{s=0}^{n-1} c_r e^{\mathrm{sign} 2\pi i r s/n} \]
\pagebreak

\[v^{n+1}=m.v^{n}\]
\pagebreak

\[v^{n+1}/=\mathrm{norm}(v^{n+1})\]
\pagebreak

$ v^{0}=\mathrm{start} $
\pagebreak

$ n$
\pagebreak

$ \mathrm{norm}(v^{n+1}-v^{n})$
\pagebreak

\[v.m.v \over v.v \]
\pagebreak

$p_v = sum_b p_{bv}$
\pagebreak

\[\sum_{b \in \rm{subset}} p_{bv} = { \sum_b p_{bv} \over \rm{numsubsets} } \]
\pagebreak

\[ \lambda^\mathrm{new} = \lambda + \zeta D \nabla \Psi \]
\pagebreak

$\Psi$
\pagebreak

$D$
\pagebreak

$\zeta$
\pagebreak

\[\sum_{b \in \mathrm{subset}} P_{bv} = \sum_b P_{bv} \over \mathrm{numsubsets} \]
\pagebreak

\[ \zeta= { \alpha \over 1+ \gamma n } \]
\pagebreak

$n$
\pagebreak

$\alpha$
\pagebreak

$\gamma$
\pagebreak

$\alpha \approx 1$
\pagebreak

$ [0, 1, -1, 2, -2, ...] $
\pagebreak

$ [0, 1, -1, 2, 3 ] $
\pagebreak

\[ P^\mathrm{full}_{bv} = \mathrm{norm}_b P^\mathrm{normalised}_{bv} \]
\pagebreak

$\mathrm{norm}_b $
\pagebreak

\[ G_v = \beta ( {\lambda_v \over F_v} - 1) \]
\pagebreak

$ \lambda$
\pagebreak

$F$
\pagebreak

$|\lambda_v| < M*|F_v| $
\pagebreak

${\lambda_v \over F_v}$
\pagebreak

$M*\rm{sign}(F_v)*\rm{sign}(lambda_v)$
\pagebreak

$M$
\pagebreak

\[ f = \sum_{dr} w_{dr} 1/scalar^2 * log(cosh(\lambda_r - \lambda_{r+dr})) * \kappa_r * \kappa_{r+dr})) \]
\pagebreak

$r$
\pagebreak

$dr$
\pagebreak

$w_{dr}$
\pagebreak

$\kappa$
\pagebreak

$ f $
\pagebreak

\[ \phi(f) = \sqrt{\alpha^2 + |\nabla f|^2 - {\langle\nabla f,\xi\rangle}^2} \]
\pagebreak

$ \xi $
\pagebreak

\[ \xi = \frac{\nabla v}{\sqrt{|\nabla v|^2 + \eta^2}} \]
\pagebreak

$ v $
\pagebreak

$ \alpha $
\pagebreak

$ \eta $
\pagebreak

$y$
\pagebreak

$\bar y$
\pagebreak

\[ L(y\;\bar y) = \sum_b y_b log \bar y_b - \mathrm{log} y_b! - \bar y_b \]
\pagebreak

$Y(\lambda)$
\pagebreak

\[ {\partial L \over \partial \lambda_v} = \sum_b \left( {y_b \over Y_b} - 1 \right) {\partial Y_b \over \partial \lambda_v } \]
\pagebreak

\[ Y = P \lambda + r \]
\pagebreak

$P_{bv}$
\pagebreak

$b$
\pagebreak

$\lambda_v$
\pagebreak

\[ {\partial L \over \partial \lambda_v} = \sum_b P_{bv} {y_b \over Y_b} - P_v \]
\pagebreak

\[ P_v = \sum_b P_{bv} \]
\pagebreak

$P_v$
\pagebreak

$r=0$
\pagebreak

$v$
\pagebreak

\[ \mathrm{KL}(y,\bar y) = \sum_b y_b \mathrm{log}(y_b/\bar y_b) + \bar y_b - y_b \]
\pagebreak

$\mathrm{KL}(y,\bar y)=0$
\pagebreak

$y=\bar y$
\pagebreak

\[ {\partial L \over \partial \lambda_v} = \sum_b P_{bv} ({y_b \over Y_b} - 1) \]
\pagebreak

\[ {\partial L \over \partial \lambda_v} + P_v = \sum_b P_{bv} {y_b \over Y_b} \]
\pagebreak

\[ \begin{array}{lcl} \Lambda_{\nu}^{(s+1)}&&=\Lambda_{\nu}^{(s)} \frac{1}{ \sum\limits_{b\in S_{l}, g} \sum\limits_{\nu'} \hat{W}^{-1} _{\nu'g\rightarrow \nu}P_{\nu' b}A_{bg}+\beta \nabla_{\Lambda_{\nu}} E_{\nu}^{(s)}}\\ &&\times \sum\limits_{b\in S_{l}, g} \sum\limits_{\nu'}\left(\hat{W}^{-1} _{\nu'g\rightarrow \nu}P_{\nu' b}\frac{Y_{bg}}{\sum\limits_{\tilde{\nu}}P_{b\tilde{\nu}}\sum\limits_{\tilde{\nu}'}\hat{W} _{\tilde{\nu}'\rightarrow \tilde{\nu}g}\Lambda_{\tilde{\nu}'}^{(s)}+\frac{B_{bg}}{A_{bg}}}\right) \end{array} \]
\pagebreak

$P$
\pagebreak

\[ P = D G \]
\pagebreak

\[ P \lambda + r = D ( F \lambda + a ) \]
\pagebreak

\[ P' y = F' D y \]
\pagebreak

$B$
\pagebreak

\[ B D \left[ y / \left( D (F \lambda + a) \right) \right] - B D 1 = B \left[ y / \left(F \lambda + a \right) \right] - B D 1 \]
\pagebreak

$a$
\pagebreak

\[ H_{jk} = - \sum_i P_{ij} h_i^{''}(y_i) P_{ik} \]
\pagebreak

\[ h_i(l) = y_i log (l) - l; h_i^{''}(y_i) = y_i / ((P \lambda)_i + a_i)^2; \]
\pagebreak

$P_{ij} $
\pagebreak

\[ h_i^{''}(y_i) \approx -1/y_i \]
\pagebreak

\[ H_{jk} = - \sum_i P_{ij}(1/y_i) P_{ik} \]
\pagebreak

\[ H_{jk} = \sum_i G_{ij}{1 \over n_i \mathrm{smooth}( n_i y_i)} G_{ik} \]
\pagebreak

$n_i$
\pagebreak

\[ P_{ij} = {1 \over n_i } G_{ij}\]
\pagebreak

$1 \over y_i+1 $
\pagebreak

\[ h_i(l) = y_i log (l) - l; h_i^{''}(y_i) = - y_i / ((P \lambda)_i + a_i)^2; \]
\pagebreak

\[ H_{jk} = - \sum_i P_{ij}(y_i / ((P \lambda)_i + a_i)^2) P_{ik} \]
\pagebreak

\[ g_r = \sum_dr w_{dr} (\lambda_r - \lambda_{r+dr}) * \kappa_r * \kappa_{r+dr} \]
\pagebreak

\[ g_r = \sum_{dr} w_{dr} * \frac{\left(\lambda_{j}-\lambda_{k}\right)\left(\gamma\left|\lambda_{j}-\lambda_{k}\right|+\lambda_{j}+3 \lambda_{k} + 2 \epsilon \right)} {\left(\lambda_{j}+\lambda_{k}+\gamma\left|\lambda_{j}-\lambda_{k}\right| + \epsilon \right)^{2}} * \kappa_r * \kappa_{r+dr} \]
\pagebreak

$\epsilon$
\pagebreak

\[ out_i = \sum_j kernelforthisdirection_j in_{i-j} \]
\pagebreak

\[ M(k,s,P) = (1 - (1 - G(k, s)^2)^{(P + 1)})/ G(k, s) \]
\pagebreak

$ G(k,s) $
\pagebreak

$G(0,s) = 1$
\pagebreak

\[ Metz(x,s,P) = Metz(x/s, 1 ,P)/s \]
\pagebreak

\[ abs(x), abs(y), abs(z) <= length_x/2, length_y/2, length_z/2 \]
\pagebreak

$r = coord - origin$
\pagebreak

\[ {(r.dir_x)^2 \over R_x^2} + {(r.dir_y)^2 \over R_y^2} + {(r.dir_z)^2 \over R_z^2} <= 1 \]
\pagebreak

$dir_x, dir_y, dir_z$
\pagebreak

\[ |r.dir_z|<L/2 \]
\pagebreak

\[ {(r.dir_x)^2 \over R_x^2} + {(r.dir_y)^2 \over R_y^2} <= 1 \]
\pagebreak

\[ \theta_1 <= atan2(r.dir_y,r.dir_x) <= \theta_2 \]
\pagebreak

\[ r' = \mathrm{conj}(q)(r-t)q \]
\pagebreak

${[}q0,qz,qy,qx{]}$
\pagebreak

${[}n_z,n_y,n_x{]}$
\pagebreak

$\phi$
\pagebreak

${[}cos(\phi),sin(\phi) n_z, sin(\phi) n_y, sin(\phi)n_x{]}$
\pagebreak

\[ \hat\kappa = \sqrt{ P^T \bigg( \frac{y}{ (P\lambda+a)^2 } \bigg) P1 } \]
\pagebreak

\[ \tilde\kappa = \sqrt{ P^T \bigg( \frac{1}{y} \bigg)P1 } \]
\pagebreak

\end{document}
